Merkle tree: working on the correctness of high-level design; changed the proof strategy

secure_api/merkle_tree/MerkleTree.New.High.Correct.fst
@@ -7,6 +7,7 @@ open MerkleTree.Spec
 open MerkleTree.New.High
 
 open FStar.Classical
+open FStar.Mul
 open FStar.Ghost
 open FStar.Seq
 
@@ -35,391 +36,145 @@ val remainder_2_1_div:
         (ensures (n / 2 + 1 = (n + 1) / 2))
 let remainder_2_1_div n = ()  
 
-// val is_pow2: n:nat -> GTot bool
-// let rec is_pow2 n =
-//   if n = 0 then false
-//   else if n = 1 then true
-//   else if n % 2 = 0 then is_pow2 (n / 2)
-//   else false
+/// Invariants of high-level Merkle tree design
 
-// val pow2_ceil: 
-//   n:nat -> GTot (c:nat{n <= pow2 c})
-// let rec pow2_ceil n =
-//   if n <= 1 then 0
-//   else 1 + pow2_ceil ((n + 1) / 2)
+val mt_hashes_lth_inv:
+  lv:nat{lv <= 32} ->
+  j:nat{j < pow2 (32 - lv)} ->
+  fhs:hash_ss{S.length fhs = 32} ->
+  GTot Type0 (decreases (32 - lv))
+let rec mt_hashes_lth_inv lv j fhs =
+  if lv = 32 then true
+  else (S.length (S.index fhs lv) == j /\
+       mt_hashes_lth_inv (lv + 1) (j / 2) fhs)
 
-// val pow2_is_pow2: 
-//   n:nat -> Lemma (is_pow2 (pow2 n)) [SMTPat (pow2 n)]
-// let rec pow2_is_pow2 n =
-//   if n = 0 then () else pow2_is_pow2 (n-1)
-
-// val pow2_ceil_inc_1:
-//   n:nat ->
-//   Lemma (requires (not (is_pow2 n)))
-//         (ensures (pow2_ceil n = pow2_ceil (n + 1)))
-// #reset-options "--z3rlimit 10"
-// let rec pow2_ceil_inc_1 n =
-//   if n <= 1 then ()
-//   else if n % 2 = 0 then pow2_ceil_inc_1 (n / 2)
-//   else (assert (pow2_ceil n = 1 + pow2_ceil ((n + 1) / 2));
-//        assert (pow2_ceil (n + 1) = 1 + pow2_ceil (n / 2 + 1)))
-
-// val pow2_ceil_inc_2:
-//   n:nat ->
-//   Lemma (requires (is_pow2 n))
-//         (ensures (pow2_ceil n + 1 = pow2_ceil (n + 1)))
-// let rec pow2_ceil_inc_2 n =
-//   if n <= 1 then ()
-//   else if n % 2 = 0 
-//   then (assert (pow2_ceil n = 1 + pow2_ceil (n / 2));
-//        assert (pow2_ceil (n + 1) = 1 + pow2_ceil (n / 2 + 1));
-//        pow2_ceil_inc_2 (n / 2))
-//   else ()
-
-/// Connection to Merkle tree specification
-
-// It is more natural to have a *relation* between a high-level Merkle tree and
-// a spec, since the high-level does not hold some elements that are never used
-// for generating Merkle paths, e.g., rightmost hashes (`MT?.rhs`). Even with
-// `MT?.rhs` the high-level design is not equal to a full Merkle tree with some
-// right paddings.
-//
-// For example, when `MT?.j = 5`, `MT?.hs` has hashes below:
-// ----------------------------|
-//       | [0] [1] [2] [3] [4] |
-// hs[2] | h03                 |
-// hs[1] | h01 h23             |
-// hs[0] | h0  h1  h2  h3  h4  |
-// -----------------------------
-// After calculating rightmost hashes, `MT?.rhs` has hashes below:
-// ------------|
-// rhs[2] | h4 |
-// rhs[1] | .  |
-// rhs[0] | .  |
-// ------------|
-// The spec has hashes and right-pads below (P is a pad):
-// ----------------------------------------|
-// spec[3] | h04                           |
-// spec[2] | h03 h4                        |
-// spec[1] | h01 h23 h4  P                 |
-// spec[0] | h0  h1  h2  h3  h4  P   P   P |
-// ----------------------------------------|
-// This is intuitively because `MT?.hs` and `MT?.rhs` have minimal required 
-// hashes to calculate Merkle paths for {h0, ..., h5}.
-//
-
-val hash_seq_lift: 
-  hs:hash_seq -> 
-  GTot (shs:MTS.hash_seq{S.length shs = S.length hs})
-       (decreases (S.length hs))
-let rec hash_seq_lift hs =
-  if S.length hs = 0 then S.empty
-  else S.cons (HRaw (S.head hs)) (hash_seq_lift (S.tail hs))
-
-val create_pads: len:nat -> GTot (pads:MTS.hash_seq{S.length pads = len})
-let create_pads len = S.create len HPad
-
-val hash_seq_spec_rel:
-  j:nat -> n:nat{j <= pow2 n} ->
-  olds:hash_seq ->
-  hs:hash_seq{S.length hs = j - S.length olds} ->
-  smt:MTS.merkle_tree n ->
+val mt_hashes_next_rel:
+  j:nat ->
+  hs:hash_seq{S.length hs = j} ->
+  nhs:hash_seq{S.length nhs = j / 2} ->
   GTot Type0
-let hash_seq_spec_rel j n olds hs smt =
-  S.equal (hash_seq_lift (S.append olds hs))
-          (S.slice smt 0 j)
+let mt_hashes_next_rel j hs nhs =
+  forall (i:nat{i < j / 2}).
+    S.index nhs i == 
+    hash_2 (S.index hs (2 * i)) (S.index hs (2 * i + 1))
 
-val hash_seq_spec_rel_equiv:
-  j:nat -> n:nat{j <= pow2 n} ->
-  olds:hash_seq ->
-  hs:hash_seq{S.length hs = j - S.length olds} ->
-  smt1:MTS.merkle_tree n -> smt2:MTS.merkle_tree n ->
-  Lemma (requires (hash_seq_spec_rel j n olds hs smt1 /\
-                  S.equal (S.slice smt1 0 j) (S.slice smt2 0 j)))
-        (ensures (hash_seq_spec_rel j n olds hs smt2))
-let hash_seq_spec_rel_equiv j n olds hs smt1 smt2 = ()
+val mt_hashes_inv:
+  lv:nat{lv < 32} ->
+  j:nat{j < pow2 (32 - lv)} ->
+  fhs:hash_ss{S.length fhs = 32 /\ mt_hashes_lth_inv lv j fhs} ->
+  GTot Type0 (decreases (32 - lv))
+let rec mt_hashes_inv lv j fhs =
+  if lv = 31 then true
+  else (mt_hashes_next_rel j (S.index fhs lv) (S.index fhs (lv + 1)) /\
+       mt_hashes_inv (lv + 1) (j / 2) fhs)
 
-val hash_ss_length_spec:
-  j:nat -> n:nat{j <= pow2 n} ->
-  olds:hash_ss{S.length olds = n} ->
-  hs:hash_ss{S.length hs = n} ->
+val merge_hs:
+  hs1:hash_ss ->
+  hs2:hash_ss{S.length hs1 = S.length hs2} ->
+  GTot (mhs:hash_ss{S.length mhs = S.length hs1})
+       (decreases (S.length hs1))
+let rec merge_hs hs1 hs2 =
+  if S.length hs1 = 0 then S.empty
+  else (S.cons (S.append (S.head hs1) (S.head hs2))
+               (merge_hs (S.tail hs1) (S.tail hs2)))
+
+val merge_hs_index:
+  hs1:hash_ss ->
+  hs2:hash_ss{S.length hs1 = S.length hs2} ->
+  i:nat{i < S.length hs1} ->
+  Lemma (requires True)
+        (ensures (S.equal (S.index (merge_hs hs1 hs2) i)
+                          (S.append (S.index hs1 i) (S.index hs2 i))))
+        (decreases (S.length hs1))
+        [SMTPat (S.index (merge_hs hs1 hs2) i)]
+let rec merge_hs_index hs1 hs2 i =
+  if S.length hs1 = 0 then ()
+  else if i = 0 then ()
+  else merge_hs_index (S.tail hs1) (S.tail hs2) (i - 1)
+
+val mt_olds_inv:
+  lv:nat{lv <= 32} ->
+  i:nat ->
+  olds:hash_ss{S.length olds = 32} ->
+  GTot Type0 (decreases (32 - lv))
+let rec mt_olds_inv lv i olds =
+  if lv = 32 then true
+  else (let ofs = offset_of i in
+       S.length (S.index olds lv) == ofs /\
+       mt_olds_inv (lv + 1) (i / 2) olds)
+
+val mt_olds_hs_lth_inv_ok:
+  lv:nat{lv <= 32} ->
+  i:nat ->
+  j:nat{i <= j /\ j < pow2 (32 - lv)} ->
+  olds:hash_ss{S.length olds = 32 /\ mt_olds_inv lv i olds} ->
+  hs:hash_ss{S.length hs = 32 /\ hs_wf_elts lv hs i j} ->
+  Lemma (requires True)
+        (ensures (mt_hashes_lth_inv lv j (merge_hs olds hs)))
+        (decreases (32 - lv))
+let rec mt_olds_hs_lth_inv_ok lv i j olds hs =
+  if lv = 32 then ()
+  else (mt_olds_hs_lth_inv_ok (lv + 1) (i / 2) (j / 2) olds hs)
+
+val mt_olds_hs_inv:
+  lv:nat{lv < 32} ->
+  i:nat ->
+  j:nat{i <= j /\ j < pow2 (32 - lv)} ->
+  olds:hash_ss{S.length olds = 32 /\ mt_olds_inv lv i olds} ->
+  hs:hash_ss{S.length hs = 32 /\ hs_wf_elts lv hs i j} ->
   GTot Type0
-let rec hash_ss_length_spec j n olds hs =
-  if n = 0 then true
-  else (S.length (S.append (S.head olds) (S.head hs)) = j /\
-       hash_ss_length_spec (j / 2) (n - 1) (S.tail olds) (S.tail hs))
+let mt_olds_hs_inv lv i j olds hs =
+  mt_olds_hs_lth_inv_ok lv i j olds hs;
+  mt_hashes_inv lv j (merge_hs olds hs)
 
-val hash_ss_spec_rel:
-  j:nat -> n:nat{j <= pow2 n} ->
-  olds:hash_ss{S.length olds = n} ->
-  hs:hash_ss{S.length hs = n /\ hash_ss_length_spec j n olds hs} ->
-  smt:MTS.merkle_tree n ->
+// joonwonc: some other invariants (e.g., about `MT?.rhs`) will be added later.
+val mt_inv: 
+  mt:merkle_tree{mt_wf_elts mt} ->
+  olds:hash_ss{S.length olds = 32 /\ mt_olds_inv 0 (MT?.i mt) olds} ->
   GTot Type0
-let rec hash_ss_spec_rel j n olds hs smt =
-  if n = 0 then true
-  else (hash_seq_spec_rel j n (S.head olds) (S.head hs) smt /\
-       hash_ss_spec_rel (j / 2) (n - 1) 
-         (S.tail olds) (S.tail hs) (mt_next_lv smt))
-
-val hash_ss_spec_rel_equiv:
-  j:nat -> n:nat{j <= pow2 n} ->
-  olds:hash_ss{S.length olds = n} ->
-  hs:hash_ss{S.length hs = n /\ hash_ss_length_spec j n olds hs} ->
-  smt1:MTS.merkle_tree n -> smt2:MTS.merkle_tree n ->
-  Lemma (requires (hash_ss_spec_rel j n olds hs smt1 /\
-                  S.equal (S.slice smt1 0 j) (S.slice smt2 0 j)))
-        (ensures (hash_ss_spec_rel j n olds hs smt2))
-let rec hash_ss_spec_rel_equiv j n olds hs smt1 smt2 =
-  if n = 0 then ()
-  else (mt_next_lv_equiv j n smt1 smt2;
-       hash_ss_spec_rel_equiv (j / 2) (n - 1) (S.tail olds) (S.tail hs)
-                              (mt_next_lv smt1) (mt_next_lv smt2))
-
-val hash_seq_lift_to_spec:
-  fhs:hash_seq ->
-  n:nat{S.length fhs <= pow2 n} ->
-  GTot (MTS.merkle_tree n)
-let hash_seq_lift_to_spec fhs n =
-  S.append (hash_seq_lift fhs) (create_pads (pow2 n - S.length fhs))
-
-val hash_seq_lift_to_spec_slice_eq:
-  fhs1:hash_seq -> fhs2:hash_seq ->
-  n:nat{S.length fhs1 <= pow2 n && S.length fhs2 <= pow2 n} ->
-  i:nat{i <= S.length fhs1 && i <= S.length fhs2} ->
-  Lemma (requires (S.equal (S.slice fhs1 0 i) (S.slice fhs2 0 i)))
-        (ensures (S.equal (S.slice (hash_seq_lift_to_spec fhs1 n) 0 i)
-                          (S.slice (hash_seq_lift_to_spec fhs2 n) 0 i)))
-let hash_seq_lift_to_spec_slice_eq fhs1 fhs2 n i =
-  admit ()
-
-val hash_ss_spec_:
-  j:nat -> n:nat{n > 0 && j <= pow2 n} ->
-  olds:hash_ss{S.length olds = n} ->
-  hs:hash_ss{S.length hs = n /\ hash_ss_length_spec j n olds hs} ->
-  GTot Type0
-let hash_ss_spec_ j n olds hs =
-  hash_ss_spec_rel j n olds hs 
-    (hash_seq_lift_to_spec (S.append (S.head olds) (S.head hs)) n)
-
-val hash_ss_spec_rec:
-  j:nat -> n:nat{n > 1 && j <= pow2 n} ->
-  olds:hash_ss{S.length olds = n} ->
-  hs:hash_ss{S.length hs = n /\ hash_ss_length_spec j n olds hs} ->
-  Lemma (requires (hash_ss_spec_ j n olds hs))
-        (ensures (hash_ss_spec_ (j / 2) (n - 1) (S.tail olds) (S.tail hs)))
-let hash_ss_spec_rec j n olds hs =
-  let spec_base = hash_seq_lift_to_spec (S.append (S.head olds) (S.head hs)) n in
-  assert (hash_seq_spec_rel (j / 2) (n - 1)
-           (S.head (S.tail olds)) (S.head (S.tail hs)) (mt_next_lv spec_base));
-  assert (S.equal (S.slice (mt_next_lv spec_base) 0 (j / 2))
-                  (S.slice (hash_seq_lift_to_spec
-                             (S.append (S.head (S.tail olds)) 
-                                       (S.head (S.tail hs))) (n - 1)) 0 (j / 2)));
-  hash_ss_spec_rel_equiv (j / 2) (n - 1) (S.tail olds) (S.tail hs)
-    (mt_next_lv spec_base)
-    (hash_seq_lift_to_spec 
-      (S.append (S.head (S.tail olds)) (S.head (S.tail hs))) (n - 1))
-
-// TODO: make a pure `exists` term for better elimination.
-val hash_ss_spec:
-  j:nat -> n:nat{j <= pow2 n} ->
-  hs:hash_ss{S.length hs = n} ->
-  GTot Type0
-let hash_ss_spec j n hs =
-  if n = 0 then True
-  else begin
-    exists (olds:hash_ss{S.length olds = n}).
-      hash_ss_length_spec j n olds hs /\
-      hash_ss_spec_ j n olds hs
-  end
-
-val hash_ss_spec_intro:
-  j:nat -> n:nat{n > 0 && j <= pow2 n} ->
-  olds:hash_ss{S.length olds = n} ->
-  hs:hash_ss{S.length hs = n /\ hash_ss_length_spec j n olds hs} ->
-  Lemma (requires (hash_ss_spec_ j n olds hs))
-        (ensures (hash_ss_spec j n hs))
-let hash_ss_spec_intro j n olds hs =
-  exists_intro
-    (fun (olds:hash_ss{S.length olds = n /\ hash_ss_length_spec j n olds hs}) ->
-      hash_ss_spec_ j n olds hs) olds
-  
-// val hash_ss_spec_elim:
-//   j:nat -> n:nat{n > 0 && j <= pow2 n} ->
-//   hs:hash_ss{S.length hs = n} ->
-//   goal:Type0 ->
-//   ex:(
-//     olds:hash_ss{S.length olds = n /\ hash_ss_length_spec j n olds hs} ->
-//     goal) ->
-//   Lemma (requires (hash_ss_spec j n hs))
-//         (ensures goal)
-// let hash_ss_spec_elim j n hs goal ex =
-
-// joonwonc: which is better: to calculate `n` from `j` or just `n = 32`?
-val mt_wf_spec: mt:merkle_tree{mt_not_empty mt} -> GTot Type0
-let mt_wf_spec mt =
-  hash_ss_spec (MT?.j mt) 32 (MT?.hs mt)
+let mt_inv mt olds =
+  mt_olds_hs_inv 0 (MT?.i mt) (MT?.j mt) olds (MT?.hs mt)
 
 /// Correctness of insertion
 
-private val seq_equal_slice_index:
-  #a:Type -> 
-  s1:S.seq a -> s2:S.seq a ->
-  n:nat -> m:nat{n <= m && m <= S.length s1 && m <= S.length s2} ->
-  i:nat{n <= i && i < m} ->
-  Lemma (requires (S.equal (S.slice s1 n m) (S.slice s2 n m)))
-        (ensures (S.index s1 i == S.index s2 i))
-private let seq_equal_slice_index #a s1 s2 n m i =
-  lemma_index_slice s1 n m (i - n);
-  lemma_index_slice s2 n m (i - n)
-
-private val seq_equal_slice_more:
-  #a:Type -> s1:S.seq a -> s2:S.seq a ->
-  n:nat -> m:nat{n <= m && m <= S.length s1 && m <= S.length s2} ->
-  k:nat{n <= k} -> l:nat{k <= l && l <= m} ->
-  Lemma (requires (S.equal (S.slice s1 n m) (S.slice s2 n m)))
-        (ensures (S.equal (S.slice s1 k l) (S.slice s2 k l)))
-private let seq_equal_slice_more #a s1 s2 n m k l =
-  slice_slice s1 n m (k - n) (l - n);
-  slice_slice s2 n m (k - n) (l - n)
-
-val hash_ss_insert_modified:
+assume val insert_hs_wf_elts:
   lv:nat{lv < 32} ->
   i:nat ->
   j:nat{i <= j /\ j < pow2 (32 - lv) - 1} ->
   hs:hash_ss{S.length hs = 32 /\ hs_wf_elts lv hs i j} ->
+  acc:hash ->
+  Lemma (requires (hs_wf_elts lv hs i j))
+        (ensures (hs_wf_elts lv (insert_ lv i j hs acc) i (j + 1)))
+
+val mt_insert_mt_wf_elts:
+  mt:merkle_tree{mt_wf_elts mt /\ mt_not_full mt} ->
   v:hash ->
-  Lemma (S.equal (S.slice hs 0 lv)
-                 (S.slice (hash_ss_insert lv i j hs v) 0 lv) /\
-        S.equal (S.slice hs (lv + 1) 32)
-                 (S.slice (hash_ss_insert lv i j hs v) (lv + 1) 32) /\
-        S.equal (S.index (hash_ss_insert lv i j hs v) lv)
-                (S.snoc (S.index hs lv) v))
-let hash_ss_insert_modified lv i j hs v = ()
+  Lemma (requires (mt_wf_elts mt))
+        (ensures (mt_wf_elts (mt_insert mt v)))
+let mt_insert_mt_wf_elts mt v =
+  insert_hs_wf_elts 0 (MT?.i mt) (MT?.j mt) (MT?.hs mt) v
 
-val insert_modified:
+val insert_inv_preserved:
   lv:nat{lv < 32} ->
   i:nat ->
   j:nat{i <= j /\ j < pow2 (32 - lv) - 1} ->
+  olds:hash_ss{S.length olds = 32 /\ mt_olds_inv lv i olds} ->
   hs:hash_ss{S.length hs = 32 /\ hs_wf_elts lv hs i j} ->
   acc:hash ->
-  Lemma (requires True)
-        (ensures (S.equal (S.slice (insert_ lv i j hs acc) 0 lv)
-                          (S.slice hs 0 lv)))
-        (decreases j)
-let rec insert_modified lv i j hs acc =
-  let ihs = hash_ss_insert lv i j hs acc in
-  hash_ss_insert_modified lv i j hs acc;
-  if j % 2 = 1
-  then (let nacc = hash_2 (S.last (S.index hs lv)) acc in
-       insert_modified (lv + 1) (i / 2) (j / 2) ihs nacc;
-       seq_equal_slice_more (insert_ (lv + 1) (i / 2) (j / 2) ihs nacc) ihs
-         0 (lv + 1) 0 lv)
-  else ()
+  Lemma (requires (mt_olds_hs_inv lv i j olds hs))
+        (ensures (insert_hs_wf_elts lv i j hs acc;
+                 mt_olds_hs_inv lv i (j + 1) olds (insert_ lv i j hs acc)))
+let rec insert_inv_preserved lv i j olds hs acc =
+  admit ()
 
-val insert_head:
-  lv:nat{lv < 32} ->
-  i:nat ->
-  j:nat{i <= j /\ j < pow2 (32 - lv) - 1} ->
-  hs:hash_ss{S.length hs = 32 /\ hs_wf_elts lv hs i j} ->
-  acc:hash ->
-  Lemma (S.equal (S.index (insert_ lv i j hs acc) lv)
-                 (S.index (hash_ss_insert lv i j hs acc) lv))
-let insert_head lv i j hs acc =
-  if j % 2 = 1
-  then (let ihs = hash_ss_insert lv i j hs acc in
-       let nacc = hash_2 (S.last (S.index hs lv)) acc in
-       assert (S.equal (S.index (insert_ lv i j hs acc) lv)
-                       (S.index (insert_ (lv + 1) (i / 2) (j / 2) ihs nacc) lv));
-       insert_modified (lv + 1) (i / 2) (j / 2) ihs nacc;
-       assert (S.equal (S.slice (insert_ (lv + 1) (i / 2) (j / 2) ihs nacc) 0 (lv + 1))
-                       (S.slice ihs 0 (lv + 1)));
-       seq_equal_slice_index
-         (insert_ (lv + 1) (i / 2) (j / 2) ihs nacc) ihs
-         0 (lv + 1) lv
-  )
-  else ()
-
-val insert_wf_spec:
-  lv:nat{lv < 32} ->
-  i:nat ->
-  j:nat{i <= j /\ j < pow2 (32 - lv) - 1} ->
-  hs:hash_ss{S.length hs = 32 /\ hs_wf_elts lv hs i j} ->
-  acc:hash ->
-  olds:hash_ss{S.length olds = 32 - lv} ->
-  Lemma (requires (hash_ss_length_spec j (32 - lv) olds (S.slice hs lv 32) /\
-                  hash_ss_spec_ j (32 - lv) olds (S.slice hs lv 32)))
-        (ensures (hash_ss_length_spec (j + 1) (32 - lv) olds
-                   (S.slice (insert_ lv i j hs acc) lv 32) /\
-                 hash_ss_spec_ (j + 1) (32 - lv) olds
-                   (S.slice (insert_ lv i j hs acc) lv 32)))
-        (decreases j)
-#reset-options "--z3rlimit 20 --max_fuel 1"
-let rec insert_wf_spec lv i j hs acc olds =
-  let ihs = insert_ lv i j hs acc in
-  insert_head lv i j hs acc;
-  hash_ss_insert_modified lv i j hs acc;
-  let spec_base = 
-    hash_seq_lift_to_spec
-      (S.append (S.head olds) (S.index hs lv)) (32 - lv) in
-
-  if j % 2 = 1
-  then begin
-    remainder_2_1_div j;
-    admit ()
-  end
-  
-  else begin
-    remainder_2_not_1_div j;
-    let ispec_base =
-      hash_seq_lift_to_spec
-        (S.append (S.head olds) (S.index ihs lv)) (32 - lv) in
-    // Since original `olds` and `hs[lv]` are unchanged after the insertion,
-    // below assertion holds.
-    assert (S.equal (S.slice (S.append (S.head olds) (S.index hs lv)) 0 j)
-                    (S.slice (S.append (S.head olds) (S.index ihs lv)) 0 j));
-    hash_seq_lift_to_spec_slice_eq
-      (S.append (S.head olds) (S.index hs lv))
-      (S.append (S.head olds) (S.index ihs lv))
-      (32 - lv) j;
-    mt_next_lv_equiv j (32 - lv) spec_base ispec_base;
-    hash_ss_spec_rel_equiv ((j + 1) / 2) (32 - (lv + 1))
-      (S.tail olds) (S.slice ihs (lv + 1) 32)
-      (mt_next_lv spec_base) (mt_next_lv ispec_base)
-  end
-
-// val mt_insert_wf_spec_0:
-//   mt:merkle_tree{mt_wf_elts mt /\ mt_empty mt} ->
-//   v:hash ->
-//   Lemma (mt_wf_spec (mt_insert mt v))
-// let mt_insert_wf_spec_0 mt v =
-//   admit ()
-
-// val mt_insert_wf_spec_1:
-//   mt:merkle_tree{mt_wf_elts mt /\ mt_not_empty mt /\ mt_not_full mt} ->
-//   v:hash ->
-//   Lemma (requires (mt_wf_spec mt))
-//         (ensures (mt_wf_spec (mt_insert mt v)))
-// let mt_insert_wf_spec_1 mt v =
-//   exists_elim
-//     (mt_wf_spec (mt_insert mt v))
-//     #(olds:hash_ss{S.length olds = 32})
-//     #(fun (olds:hash_ss{S.length olds = 32}) ->
-//         hash_ss_length_spec (MT?.j mt) 32 olds (MT?.hs mt) /\
-//         hash_ss_spec_ (MT?.j mt) 32 olds (MT?.hs mt))
-//     (mt_wf_spec mt)
-//     (fun olds -> 
-//       insert_wf_spec 0 (MT?.i mt) (MT?.j mt) (MT?.hs mt) v olds)
-
-// val mt_insert_wf_spec:
-//   mt:merkle_tree{mt_wf_elts mt /\ mt_not_full mt} ->
-//   v:hash ->
-//   Lemma (requires (mt_empty mt \/ mt_wf_spec mt))
-//         (ensures (mt_wf_spec (mt_insert mt v)))
-// let mt_insert_wf_spec mt v =
-//   if mt_empty mt
-//   then mt_insert_wf_spec_0 mt v
-//   else mt_insert_wf_spec_1 mt v
+val mt_insert_inv_preserved:
+  mt:merkle_tree{mt_wf_elts mt /\ mt_not_full mt} -> v:hash ->
+  olds:hash_ss{S.length olds = 32 /\ mt_olds_inv 0 (MT?.i mt) olds} ->
+  Lemma (requires (mt_inv mt olds))
+        (ensures (mt_insert_mt_wf_elts mt v;
+                 mt_inv (mt_insert mt v) olds))
+let mt_insert_inv_preserved mt v olds =
+  insert_inv_preserved 0 (MT?.i mt) (MT?.j mt) olds (MT?.hs mt) v
 
 /// Correctness of `mt_get_root` and `mt_get_path`
 
